Antitraces and prefix closure

Models/Prefix_Language.thy
@@ -2,14 +2,12 @@ theory Prefix_Language
   imports Language
 begin
 
-datatype 'a plist = Term "'a list" | Inf "'a stream" | Pre "'a list"
+datatype 'a plist = Trace "'a llist" | Pre "'a llist"
 
 fun pappend :: "'a plist \<Rightarrow> 'a plist \<Rightarrow> 'a plist" where
   "pappend (Pre xs) ys = Pre xs"
-| "pappend (Term xs) (Pre ys) = Pre (xs @ ys)"
-| "pappend (Term xs) (Inf ys) = Inf (xs @- ys)"
-| "pappend (Term xs) (Term ys) = Term (xs @ ys)"
-| "pappend (Inf xs) ys = Inf xs"
+| "pappend (Trace xs) (Pre ys) = Pre (xs \<frown> ys)"
+| "pappend (Trace xs) (Trace ys) = Trace (xs \<frown> ys)"
 
 lemma pappend_assoc: "pappend (pappend xs ys) zs = pappend xs (pappend ys zs)"
   apply (cases xs)
@@ -17,18 +15,54 @@ lemma pappend_assoc: "pappend (pappend xs ys) zs = pappend xs (pappend ys zs)"
   apply (cases ys)
   apply simp_all
   apply (cases zs)
-  by simp_all
+  apply simp_all
+  by (metis lappend_assoc)+
 
 type_synonym 'a plan = "'a plist set"
 
+primrec pclose :: "'a plist \<Rightarrow> 'a plan" where
+  "pclose (Trace xs') = insert (Trace xs') {Pre xs |xs. lprefix xs xs'}"
+| "pclose (Pre xs') = {Pre xs |xs. lprefix xs xs'}"
+
+definition pclosure :: "'a plan \<Rightarrow> 'a plan" ("_\<^sup>\<dagger>" [1000] 1000) where
+  "pclosure X = \<Union>(pclose ` X)"
+
+lemma pclose_trans: "xs \<in> pclose ys \<Longrightarrow> ys \<in> pclose zs \<Longrightarrow> xs \<in> pclose zs"
+  apply (cases ys)
+  apply simp_all
+  apply (cases zs)
+  apply simp_all
+  apply (cases zs)
+  apply (simp_all)
+  by (metis lprefix_trans)+
+
+lemma pclose_refl: "xs \<in> pclose xs"
+  by (cases xs) simp_all
+
+lemma pc_idem: "X\<^sup>\<dagger>\<^sup>\<dagger> = X\<^sup>\<dagger>"
+  apply (auto simp add: pclosure_def)
+  apply (rename_tac xs zs ys)
+  apply (rule_tac x = zs in bexI)
+  apply (metis pclose_trans)
+  apply simp
+  apply (rename_tac xs ys)
+  apply (rule_tac x = ys in bexI)
+  apply simp_all
+  apply (rule_tac x = xs in bexI)
+  apply simp_all
+  by (rule pclose_refl)
+
+lemma "X \<le> X\<^sup>\<dagger>"
+  by (auto simp add: pclosure_def) (metis pclose_refl)
+
+lemma "X \<le> Y \<Longrightarrow> X\<^sup>\<dagger> \<le> Y\<^sup>\<dagger>"
+  by (auto simp add: pclosure_def)
+
 primrec pterm :: "'a plist \<Rightarrow> bool" where
   "pterm (Pre xs) = False"
-| "pterm (Term xs) = True"
-| "pterm (Inf xs) = False"
+| "pterm (Trace xs) = lfinite xs"
 
-no_notation Language.l_prod (infixl "\<cdot>" 80)
-
-definition pprod :: "'a plan \<Rightarrow> 'a plan \<Rightarrow> 'a plan" (infixl "\<cdot>" 80) where
+definition pprod :: "'a plan \<Rightarrow> 'a plan \<Rightarrow> 'a plan" (infixl "\<bowtie>" 80) where
   "pprod X Y = {pappend xs ys |xs ys. xs \<in> X \<and> pterm xs \<and> ys \<in> Y} \<union> {xs. xs \<in> X \<and> \<not> pterm xs}"
 
 lemma pterm_pappend: "pterm (pappend xs ys) \<longleftrightarrow> (pterm xs \<and> pterm ys)"
@@ -37,16 +71,43 @@ lemma pterm_pappend: "pterm (pappend xs ys) \<longleftrightarrow> (pterm xs \<an
   apply (cases ys)
   by simp_all
 
-lemma pprod_assoc: "(X \<cdot> Y) \<cdot> Z = X \<cdot> (Y \<cdot> Z)"
+lemma pprod_assoc: "(X \<bowtie> Y) \<bowtie> Z = X \<bowtie> (Y \<bowtie> Z)"
   apply (simp add: pprod_def)
   apply safe
   by (metis pappend_assoc pterm_pappend)+
 
+lemma pprod_inf_dist: "(\<Union> \<XX>) \<bowtie> Y = \<Union>{X \<bowtie> Y |X. X \<in> \<XX>}"
+  by (auto simp add: pprod_def)
+
+(*
+lemma "(Trace ` X)\<^sup>\<dagger> \<bowtie> (Trace ` Y)\<^sup>\<dagger> = (Trace ` (X \<cdot> Y))\<^sup>\<dagger>"
+proof -
+  have "(Trace ` X)\<^sup>\<dagger> \<bowtie> (Trace ` Y)\<^sup>\<dagger> = \<Union>(pclose ` Trace ` X) \<bowtie> \<Union>(pclose ` Trace ` Y)"
+    by (simp add: pclosure_def)
+  also have "... = \<Union>{X' \<bowtie> \<Union>(pclose ` Trace ` Y) |X'. X' \<in> pclose ` Trace ` X}"
+    by (subst pprod_inf_dist) simp
+  also have "... = \<Union>(pclose ` Trace ` (X \<cdot> Y))"
+    apply (rule arg_cong) back
+    apply (simp add: l_prod_def pprod_def image_def)
+    apply safe
+    sledgehammer
+    apply (rule_tac x
+*)
+
 find_consts "'a llist \<Rightarrow> 'a stream"
+
+lemma "{Pre (list_of xs) |xs. lfinite xs \<and> lprefix xs xs'}"
 
 fun pshuffle_words :: "'a plist \<Rightarrow> 'b plist \<Rightarrow> ('a + 'b) plan" (infix "\<sha>" 75) where
   "(Pre xs) \<sha> (Pre ys) = Pre ` list_of ` (llist_of xs \<sha> llist_of ys)"
 | "(Term xs) \<sha> (Term ys) = Term ` list_of ` (llist_of xs \<sha> llist_of ys)"
 | "(Inf xs) \<sha> (Inf ys) = Inf ` stream_of_llist ` (llist_of_stream xs \<sha> llist_of_stream ys)"
+| "(Term xs) \<sha> (Inf ys) = Inf ` stream_of_llist ` (llist_of xs \<sha> llist_of_stream ys)"
+| "(Inf xs) \<sha> (Term ys) = Inf ` stream_of_llist ` (llist_of_stream xs \<sha> llist_of ys)"
+| "(Pre xs) \<sha> (Term ys) = Pre ` list_of ` (llist_of xs \<sha> llist_of ys)"
+| "(Term xs) \<sha> (Pre ys) = Pre ` list_of ` (llist_of xs \<sha> llist_of ys)"
+| "pshuffle_words xs ys = {}"
+
+
 
 end
